json/Utf8.v
@@ -1,96 +1,10 @@
 From Coq Require Import Strings.String.
 From Coq Require Import Strings.Ascii.
-From Coq Require Import ZArith.
+From Coq Require Import Strings.Byte.
 
 From Coq Require Import Lists.List. Import ListNotations.
 
-From Coq Require Import Strings.Byte.
-
-Open Scope char_scope.
-  
-Inductive result {T E: Type} : Type :=
-| Ok (x: T) : @result T E
-| Err (err: E) : @result T E.
-
-Arguments Ok {T E}.
-Arguments Err {T E}.
-
-Definition bind {A B E} (r: @result A E) (f: A -> @result B E) :=
-  match r with
-  | Ok p => f p
-  | Err err => Err err
-  end.
-
-Notation "'let*' p ':=' c1 'in' c2" :=
-  (bind c1 (fun p => c2))
-    (at level 61, p as pattern, c1 at next level, right associativity).
-
-Definition fmap { A B E } (f: A -> B) (r: @result A E) : @result B E :=
-  bind r (fun x => Ok (f x)).
-
-Definition parser (T: Type) {I E: Type} := list I -> @result (T * (list I)) (list E).
-
-Definition parser_map {A B I E} (f: A -> B) (p: @parser A I E) : @parser B I E :=
-  fun s =>
-    let* (x, rest) := p s in
-    Ok (f x, rest).
-
-Definition maybe {A I E} (p: @parser A I E) : @parser (option A) I E :=
-  fun s =>
-    match p s with
-    | Ok (x, rest) => Ok (Some x, rest)
-    | Err _        => Ok (None, s)
-    end.
-
-Fixpoint any_aux {A I E} (parsers: list (@parser A I E)) (errs: list E) : @parser A I E :=
-  fun s =>
-    match parsers with
-    | [] => Err errs
-    | p :: rest =>
-        match p s with
-        | Err err => any_aux rest (err ++ errs) s
-        | Ok p => Ok p
-        end
-    end.
-
-Definition any {A I E} (parsers : list (@parser A I E)): @parser A I E := any_aux parsers [].
-
-Definition predicate {I E} (pred: I -> bool) (err: option I -> E) : @parser I I E :=
-  fun s => 
-    match s with
-    | [] => Err [ err None ]
-    | c :: rest =>
-        match pred c with
-        | true => Ok (c, rest)
-        | false => Err [ err (Some c) ]
-        end
-    end.
-
-Fixpoint many_aux { A I E} (p: @parser A I E) (fuel: nat) : @parser (list A) I E :=
-  fun s => 
-    match fuel with
-    | 0 => Ok ([], s)
-    | S fuel' =>
-        match p s with
-        | Err _ => Ok ([], s)
-        | Ok (val, rest) =>
-            let* (vals, rest) := many_aux p fuel' rest in
-            Ok (val :: vals, rest)
-        end
-    end.
-
-Definition many {A I E} (p: @parser A I E): @parser (list A) I E :=
-  fun s => many_aux p (S (length s)) s.
-
-(* Fixpoint repeat_n {T I E} (n: nat) (p: @parser T I E) : @parser (Vector.t T n) I E := *)
-(*   fun s => *)
-(*     match n with *)
-(*     | 0 => Ok (nil T, s) *)
-(*     | S n' => *)
-(*         let* (val, rest) := p s in *)
-(*         let* (vals, rest) := repeat_n n' p rest in *)
-(*         Ok (cons T val n' vals, rest) *)
-(*     end. *)
+Require Import Json.Parser.
 
 (* ============================================== *)
 (* UTF-8 encoding and decoding                    *)
@@ -112,7 +26,7 @@ Open Scope bool_scope.
 Definition b4_equal (a b: b4) : bool :=
   let '(a1, a2, a3, a4) := a in
   let '(b1, b2, b3, b4) := b in
-  (xorb a1 b1) && (xorb a2 b2) && (xorb a3 b3) && (xorb a4 b4).
+  (Bool.eqb a1 b1) && (Bool.eqb a2 b2) && (Bool.eqb a3 b3) && (Bool.eqb a4 b4).
 
 Inductive hex : Type :=
 | H0 | H1 | H2 | H3
@@ -167,10 +81,9 @@ Inductive codepoint_range :=
 | FourthRange (fst: b3) (snd: b6) (trd: b6) (frth: b6).
 
 Inductive unicode_error :=
-| UnicodeUnexpectedEOF
 | OverlongEncoding (cr: codepoint_range)
-| InvalidContinuationHeader (x: byte)
-| InvalidStartHeader (x: byte)
+| InvalidContinuationHeader (x: option byte)
+| InvalidStartHeader (x: option byte)
 | IllegalSurrogatePair
 | IllegalCodepoint.
 
@@ -210,7 +123,7 @@ Definition codepoint_range_to_codepoint (cr: codepoint_range) : option codepoint
 Definition codepoint_eqb (a b: codepoint) : bool :=
   let '(a1, a2, a3, a4, a5, a6) := a in
   let '(b1, b2, b3, b4, b5, b6) := b in
-  (xorb a1 b1) && b4_equal a2 b2 && b4_equal a3 b3 && b4_equal a4 b4 && b4_equal a5 b5 && b4_equal a6 b6.
+  (Bool.eqb a1 b1) && b4_equal a2 b2 && b4_equal a3 b3 && b4_equal a4 b4 && b4_equal a5 b5 && b4_equal a6 b6.
 
 Definition from_ascii (c: ascii) : codepoint :=
   let '(b1, (b2, (b3, (b4, (b5, (b6, (b7, _))))))) := to_bits (byte_of_ascii c) in
@@ -245,20 +158,15 @@ Definition parse_continuation : @parser b6 byte unicode_error :=
     fun (b: byte) =>
       let '(b1, (b2, (b3, (b4, (b5, (b6, (b7, b8))))))) := to_bits b in
       andb b8 (negb b7) in
-  let handle_err_char :=
-    fun c => match c with
-          | Some c' => InvalidContinuationHeader c'
-          | None => UnicodeUnexpectedEOF
-          end in
-  parser_map continuation_from_byte (predicate is_continuation handle_err_char).
+  parser_map continuation_from_byte (predicate is_continuation InvalidContinuationHeader).
 
 Definition parse_header : @parser encoding_size byte unicode_error :=
   fun s =>
     match s with
-    | [] => Err [ UnicodeUnexpectedEOF ]
+    | [] => Err (Error (InvalidStartHeader None))
     | h :: rest =>
         match encoding_size_from_header h with
-        | None => Err [ InvalidStartHeader h ]
+        | None => Err (Error (InvalidStartHeader (Some h)))
         | Some e => Ok (e, rest)
         end
     end.
@@ -284,7 +192,7 @@ Definition parse_codepoint : @parser codepoint byte unicode_error :=
       end in
     match codepoint_range_to_codepoint codepoint_bits with
     | Some code => Ok (code, rest)
-    | None      => Err [ OverlongEncoding codepoint_bits ]
+    | None      => Err (Error (OverlongEncoding codepoint_bits))
     end.
 
 Definition utf8_decode : @parser unicode_str byte unicode_error :=
@@ -339,7 +247,7 @@ Definition test4 :
   reflexivity.
 Qed.
 
-Definition to_unicode (s: string) : @result unicode_str (list unicode_error) :=
+Definition to_unicode (s: string) : @result unicode_str (@error unicode_error) :=
   let bytes := List.map byte_of_ascii (list_ascii_of_string s) in
   fmap (fun '(v, _) => v) (utf8_decode bytes).
 
@@ -363,179 +271,3 @@ Definition utf8_encode_codepoint (c: codepoint) : list byte :=
 
 Definition utf8_encode (s: unicode_str) : list byte :=
   concat (List.map utf8_encode_codepoint s).
-
-(* ============================================== *)
-(* JSON parser implementation                     *)
-(* ============================================== *)
-
-Inductive nonzero :=
-| D1 | D2 | D3
-| D4 | D5 | D6
-| D7 | D8 | D9.
-
-Inductive digit :=
-| Zero
-| NonZero : nonzero -> digit.
-
-Inductive sign :=
-| Positive
-| Negative.
-
-Inductive integer :=
-| IntegerZero
-| MoreThanZero (first_digit: nonzero) (rest_digits: list digit).
-
-Record exponent := {
-    exponent_sign: option sign;
-    first_digit: digit;
-    digits: list digit
-  }.
-
-Record number := {
-    negative: bool;
-    integer_part: integer;
-    fractional_part: list digit;
-    exponent_part: option exponent
-  }.
-
-Inductive error_message :=
-| UnexpectedEOF
-| UnexpectedChar (c: codepoint)
-| ExpectedChar (c: codepoint) (got: codepoint).
-
-Inductive json : Type :=
-| JNull
-| JTrue
-| JFalse
-| JNumber (n: number)
-| JString (s: unicode_str)
-| JList   (l: list json)
-| JObject (obj: list (unicode_str * json)).
-
-Definition json_parser (T: Type) := @parser T codepoint error_message.
-
-Definition expect (c: ascii) : json_parser codepoint :=
-  predicate (codepoint_eqb (from_ascii c))
-    (fun c' => match c' with
-            | Some c' => UnexpectedChar c'
-            | None   => UnexpectedEOF
-            end).
-
-Definition not (c: ascii) : json_parser codepoint :=
-  predicate (fun c' => negb (codepoint_eqb (from_ascii c) c'))
-    (fun c' => match c' with
-            | Some c' => ExpectedChar (from_ascii c) c'
-            | None => UnexpectedEOF
-            end).
-
-Definition parse_nonzero : json_parser nonzero :=
-  let p digit char := parser_map (fun _ => digit) (expect char) in
-  any [
-      p D1 "1"; p D2 "2"; p D3 "3";
-      p D4 "4"; p D5 "5"; p D6 "6";
-      p D7 "7"; p D8 "8"; p D9 "9"
-    ].
-
-Definition parse_digit : json_parser digit :=
-  let z := parser_map (fun _ => Zero) (expect "0") in
-  let n := parser_map NonZero parse_nonzero in
-  any [z; n].
-
-Definition parse_integer : json_parser integer :=
-  let parse_integer_zero := parser_map (fun _ => IntegerZero) (expect "0") in
-  let parse_more_than_zero :=
-    fun s =>
-      let* (fst, rest) := parse_nonzero s in
-      let* (rest_digits, rest) := many parse_digit rest in
-      Ok (MoreThanZero fst rest_digits, rest) in
-  any [ parse_integer_zero; parse_more_than_zero ].
-
-Definition parse_fraction: json_parser (list digit) :=
-  fun s =>
-    let* (_dot, rest) := expect "." s in
-    let* (digits, rest) := many parse_digit rest in
-    Ok (digits, rest).
-
-Definition parse_sign : json_parser sign :=
-  any [ parser_map (fun _ => Negative) (expect "-");
-        parser_map (fun _ => Positive) (expect "+") ].
-
-Definition parse_exponent: json_parser exponent :=
-  fun s =>
-    let* (_e, rest) := any [ expect "e"; expect "E" ] s in
-    let* (sign, rest) := maybe parse_sign rest in
-    let* (fst_digit, rest) := parse_digit rest in
-    let* (digits, rest) := many parse_digit rest in
-    Ok( {| exponent_sign := sign; digits:= digits; first_digit:= fst_digit |}, rest).
-
-Definition parse_number: json_parser number :=
-  fun s =>
-    let* (negative, rest) := maybe (expect "-") s      in
-    let* (integer, rest)  := parse_integer rest        in
-    let* (fraction, rest) := maybe parse_fraction rest in
-    let* (exponent, rest) := maybe parse_exponent rest in
-    Ok({|
-          negative := match negative with Some _ => true | None => false end;
-          integer_part := integer;
-          fractional_part := match fraction with Some l => l | None => [] end;
-          exponent_part := exponent
-        |}, rest).
-
-Definition number_str : unicode_str.
-  refine (
-      let str := to_unicode "1"%string in
-      (match str as e return e = to_unicode "1"%string -> unicode_str with
-       | Ok v => fun H => v
-       | Err e => fun H => _
-       end) (eq_refl str)).
-  unfold to_unicode in H.
-  discriminate.
-Defined.
-
-Compute (parse_number number_str).
-
-
-(* Definition serialize_json (obj: json) : unicode_str := *)
-(*   match obj with *)
-(*   | JNull => "null" *)
-(*   | JTrue => "true" *)
-(*   | JFalse => "false" *)
-(*   | JNumber n => string_of_nat n *)
-(*   | JString s => String "034"%char (s ++ (String "034"%char EmptyString)) *)
-(*   | _ => "" *)
-(*   end. *)
-
-(* Compute (serialize_json (JString "hello world")). *)
-(* Close Scope string_scope. *)
-
-(* Definition parse_constant (c: json) : json_parser json := *)
-(*   let const_string := serialize_json c in  *)
-(*   fun s => *)
-(*     if prefix const_string s then *)
-(*       Ok((c, substring (String.length const_string) (String.length s) s)) *)
-(*     else *)
-(*       Err (Message "Expected " ++ const_string). *)
-                        
-(* Definition parse_null: json_parser json := parse_constant JNull. *)
-(* Definition parse_true: json_parser json := parse_constant JTrue. *)
-(* Definition parse_false: json_parser json := parse_constant JFalse. *)
-
-(* Definition parse_string: json_parser json := *)
-(*   fun s => *)
-(*     let* (_, rest) := expect """" s in *)
-(*     let* (s, rest) := many (not """") rest in *)
-(*     let* (_, rest) := expect """" rest in *)
-(*     Ok (JString (string_of_list_ascii (rev s)), rest). *)
-
-(* Definition parse_object_aux (fuel: nat) (acc: list (string * json)) : json_parser json :=  *)
-
-(* Definition parse_object: json_parser json :=  *)
-
-(* Definition parse_value : json_parser json := *)
-(*   any [ *)
-(*       parse_number; *)
-(*       parse_string; *)
-(*       parse_null; *)
-(*       parse_true; *)
-(*       parse_false *)
-(*     ]. *)
