json/Json.v
@@ -1,0 +1,273 @@
+From Coq Require Import Strings.String.
+From Coq Require Import Strings.Ascii.
+From Coq Require Import ZArith.
+From Coq Require Import Strings.Byte.
+From Coq Require Import Lists.List. Import ListNotations.
+
+Open Scope char_scope.
+
+Require Import Json.Parser.
+Require Import Json.Utf8.
+
+Local Notation "0" := false.
+Local Notation "1" := true.
+
+(* ============================================== *)
+(* JSON parser implementation                     *)
+(* ============================================== *)
+
+Inductive nonzero :=
+| D1 | D2 | D3
+| D4 | D5 | D6
+| D7 | D8 | D9.
+
+Inductive digit :=
+| Zero
+| NonZero (n: nonzero).
+
+Inductive sign :=
+| Positive
+| Negative.
+
+Inductive integer :=
+| IntegerZero
+| MoreThanZero (first_digit: nonzero) (rest_digits: list digit).
+
+Inductive exp_indicator :=
+| Lowercase
+| Uppercase.
+
+Record exponent := {
+    indicator: exp_indicator;
+    exponent_sign: option sign;
+    first_digit: digit;
+    digits: list digit
+  }.
+
+Record fraction := {
+    fst: digit;
+    rest_digits: list digit;
+  }.
+
+Record number := {
+    negative: bool;
+    integer_part: integer;
+    fractional_part: option fraction;
+    exponent_part: option exponent
+  }.
+
+Inductive error_message :=
+| ExpectedNonZero (got: option codepoint)
+| ExpectedDigit (got: option codepoint)
+| UnexpectedChar (c: option codepoint)
+| ExpectedChar (c: codepoint) (got: option codepoint).
+
+Inductive json : Type :=
+| JNull
+| JTrue
+| JFalse
+| JNumber (n: number)
+| JString (s: unicode_str)
+| JList   (l: list json)
+| JObject (obj: list (unicode_str * json)).
+
+Definition json_parser (T: Type) := @parser T codepoint error_message.
+
+Definition expect (c: ascii) : json_parser codepoint :=
+  predicate (codepoint_eqb (from_ascii c)) UnexpectedChar.
+
+Definition not (c: ascii) : json_parser codepoint :=
+  predicate (fun c' => negb (codepoint_eqb (from_ascii c) c')) (ExpectedChar (from_ascii c)).
+
+Compute (from_ascii "0").
+
+Definition parse_nonzero : json_parser nonzero :=
+  fun s =>
+    match s with
+    | ((0, (0, 0, 0, 0), (0, 0, 0, 0), (0, 0, 0, 0), (0, 0, 1, 1), (0, 0, 0, 1)) :: rest) => Ok (D1, rest)
+    | ((0, (0, 0, 0, 0), (0, 0, 0, 0), (0, 0, 0, 0), (0, 0, 1, 1), (0, 0, 1, 0)) :: rest) => Ok (D2, rest)
+    | ((0, (0, 0, 0, 0), (0, 0, 0, 0), (0, 0, 0, 0), (0, 0, 1, 1), (0, 0, 1, 1)) :: rest) => Ok (D3, rest)
+    | ((0, (0, 0, 0, 0), (0, 0, 0, 0), (0, 0, 0, 0), (0, 0, 1, 1), (0, 1, 0, 0)) :: rest) => Ok (D4, rest)
+    | ((0, (0, 0, 0, 0), (0, 0, 0, 0), (0, 0, 0, 0), (0, 0, 1, 1), (0, 1, 0, 1)) :: rest) => Ok (D5, rest)
+    | ((0, (0, 0, 0, 0), (0, 0, 0, 0), (0, 0, 0, 0), (0, 0, 1, 1), (0, 1, 1, 0)) :: rest) => Ok (D6, rest)
+    | ((0, (0, 0, 0, 0), (0, 0, 0, 0), (0, 0, 0, 0), (0, 0, 1, 1), (0, 1, 1, 1)) :: rest) => Ok (D7, rest)
+    | ((0, (0, 0, 0, 0), (0, 0, 0, 0), (0, 0, 0, 0), (0, 0, 1, 1), (1, 0, 0, 0)) :: rest) => Ok (D8, rest)
+    | ((0, (0, 0, 0, 0), (0, 0, 0, 0), (0, 0, 0, 0), (0, 0, 1, 1), (1, 0, 0, 1)) :: rest) => Ok (D9, rest)
+    | c :: rest => Err (Error (ExpectedNonZero (Some c)))
+    | [] => Err (Error (ExpectedNonZero None))
+    end.
+
+Definition parse_digit : json_parser digit :=
+  fun s =>
+    match s with
+    | ((0, (0, 0, 0, 0), (0, 0, 0, 0), (0, 0, 0, 0), (0, 0, 1, 1), (0, 0, 0, 0)) :: rest) => Ok (Zero, rest)
+    | other =>
+        match parse_nonzero other with
+        | Ok (d, rest) => Ok (NonZero d, rest)
+        | Err err => Err (Error (ExpectedDigit (hd_error other)))
+        end
+    end.
+
+Definition parse_integer : json_parser integer :=
+  let parse_integer_zero := parser_map (fun _ => IntegerZero) (expect "0") in
+  let parse_more_than_zero :=
+    fun s =>
+      let* (fst, rest) := parse_nonzero s in
+      let* (rest_digits, rest) := many parse_digit rest in
+      Ok (MoreThanZero fst rest_digits, rest) in
+  any [ parse_integer_zero; parse_more_than_zero ].
+
+Definition parse_fraction: json_parser fraction :=
+  fun s =>
+    let* (_dot, rest) := expect "." s in
+    let* (fst, rest) := parse_digit rest in
+    let* (digits, rest) := many parse_digit rest in
+    Ok ({| fst:= fst; rest_digits:= digits |}, rest).
+
+Definition parse_sign : json_parser sign :=
+  any [ parser_map (fun _ => Negative) (expect "-");
+        parser_map (fun _ => Positive) (expect "+") ].
+
+Definition parse_exponent: json_parser exponent :=
+  fun s =>
+    let* (e, rest) := any [ parser_map (fun _ => Lowercase) (expect "e");
+                            parser_map (fun _ => Uppercase) (expect "E") ] s in
+    let* (sign, rest) := maybe parse_sign rest in
+    let* (fst_digit, rest) := parse_digit rest in
+    let* (digits, rest) := many parse_digit rest in
+    Ok( {| indicator := e; exponent_sign := sign; digits:= digits; first_digit:= fst_digit |}, rest).
+
+Definition parse_number: json_parser number :=
+  fun s =>
+    let* (negative, rest) := maybe (expect "-") s      in
+    let* (integer, rest)  := parse_integer rest        in
+    let* (fraction, rest) := maybe parse_fraction rest in
+    let* (exponent, rest) := maybe parse_exponent rest in
+    Ok({|
+          negative := match negative with Some _ => true | None => false end;
+          integer_part := integer;
+          fractional_part := fraction;
+          exponent_part := exponent
+        |}, rest).
+
+Definition map_or {A B: Type} (f: A -> B) (opt: option A) (default: B) : B :=
+  match opt with Some c => f c | None => default end.
+
+Definition serialize_nonzero (n: nonzero) : codepoint :=
+  match n with
+  | D1 => from_ascii "1"
+  | D2 => from_ascii "2"
+  | D3 => from_ascii "3"
+  | D4 => from_ascii "4"
+  | D5 => from_ascii "5"
+  | D6 => from_ascii "6"
+  | D7 => from_ascii "7"
+  | D8 => from_ascii "8"
+  | D9 => from_ascii "9"
+  end.
+
+Definition serialize_digit (d: digit) : codepoint :=
+  match d with
+  | Zero => from_ascii "0"
+  | NonZero nz => serialize_nonzero nz
+  end.
+
+
+Definition serialize_integer (int: integer) : unicode_str :=
+  match int with
+  | IntegerZero => [(from_ascii "0")]
+  | MoreThanZero fst rest => (serialize_nonzero fst) :: (map serialize_digit rest)
+  end.
+
+Definition serialize_sign (s: sign) : codepoint :=
+  from_ascii match s with
+  | Positive => "+"
+  | Negative => "-"
+  end.
+
+Definition serialize_fraction (frac: fraction) : unicode_str :=
+  [ (from_ascii "."); serialize_digit frac.(fst) ] ++ (map serialize_digit frac.(rest_digits)).
+
+Definition serialize_exponent (exp: exponent) : unicode_str :=
+  let indicator := from_ascii match exp.(indicator) with Lowercase => "e"| Uppercase => "E" end in
+  let sign := match exp.(exponent_sign) with
+              | Some s => [serialize_sign s]
+              | None => []
+              end in
+  [ indicator ] ++ sign ++ [serialize_digit exp.(first_digit) ] ++ (map serialize_digit exp.(digits)).
+
+Definition serialize_number (num: number) : unicode_str :=
+  let sign := if num.(negative) then [ from_ascii "-" ] else [] in
+  let integer_part := serialize_integer num.(integer_part) in
+  let frac_part := map_or serialize_fraction num.(fractional_part) [] in
+  let exponent := map_or serialize_exponent num.(exponent_part) [] in
+  sign ++ integer_part ++ frac_part ++ exponent.
+
+Definition number_str : unicode_str.
+  refine (
+      let str := to_unicode "-123e-999"%string in
+      (match str as e return e = to_unicode "-123e-999"%string -> unicode_str with
+       | Ok v => fun H => v
+       | Err e => fun H => _
+       end) (eq_refl str)).
+  unfold to_unicode in H.
+  discriminate.
+Defined.
+
+Compute (utf8_encode (serialize_number {|
+            negative := 1;
+            integer_part := MoreThanZero D1 [NonZero D2; NonZero D3];
+            fractional_part := None;
+            exponent_part :=
+              Some
+                {|
+                  indicator := Lowercase;
+                  exponent_sign := Some Negative;
+                  first_digit := NonZero D9;
+                  digits := [NonZero D9; NonZero D9]
+                |}
+          |})).
+
+Definition serialize_json (obj: json) : unicode_str :=
+  match obj with
+  | JNull => to_unicode "null"%string
+  | JTrue => to_unicode "true"%string
+  | JFalse => to_unicode "false"%string
+  (* | JNumber n => string_of_nat n *)
+  (* | JString s => String "034"%char (s ++ (String "034"%char EmptyString)) *)
+  | _ => to_unicode ""%string
+  end.
+
+(* Close Scope string_scope. *)
+
+(* Definition parse_constant (c: json) : json_parser json := *)
+(*   let const_string := serialize_json c in  *)
+(*   fun s => *)
+(*     if prefix const_string s then *)
+(*       Ok((c, substring (String.length const_string) (String.length s) s)) *)
+(*     else *)
+(*       Err (Message "Expected " ++ const_string). *)
+                        
+(* Definition parse_null: json_parser json := parse_constant JNull. *)
+(* Definition parse_true: json_parser json := parse_constant JTrue. *)
+(* Definition parse_false: json_parser json := parse_constant JFalse. *)
+
+(* Definition parse_string: json_parser json := *)
+(*   fun s => *)
+(*     let* (_, rest) := expect """" s in *)
+(*     let* (s, rest) := many (not """") rest in *)
+(*     let* (_, rest) := expect """" rest in *)
+(*     Ok (JString (string_of_list_ascii (rev s)), rest). *)
+
+(* Definition parse_object_aux (fuel: nat) (acc: list (string * json)) : json_parser json :=  *)
+
+(* Definition parse_object: json_parser json :=  *)
+
+(* Definition parse_value : json_parser json := *)
+(*   any [ *)
+(*       parse_number; *)
+(*       parse_string; *)
+(*       parse_null; *)
+(*       parse_true; *)
+(*       parse_false *)
+(*     ]. *)
