json/Parser.v
@@ -1,0 +1,90 @@
+From Coq Require Import Lists.List. Import ListNotations.
+
+Inductive result {T E: Type} : Type :=
+| Ok (x: T) : @result T E
+| Err (err: E) : @result T E.
+
+Arguments Ok {T E}.
+Arguments Err {T E}.
+
+Definition bind {A B E} (r: @result A E) (f: A -> @result B E) :=
+  match r with
+  | Ok p => f p
+  | Err err => Err err
+  end.
+
+Notation "'let*' p ':=' c1 'in' c2" :=
+  (bind c1 (fun p => c2))
+    (at level 61, p as pattern, c1 at next level, right associativity).
+
+Definition fmap { A B E } (f: A -> B) (r: @result A E) : @result B E :=
+  bind r (fun x => Ok (f x)).
+
+Inductive error {E: Type}: Type :=
+| NoError
+| Error (e: E)
+| Both (left: @error E) (right: @error E).
+
+Definition parser (T: Type) {I E: Type} := list I -> @result (T * (list I)) (@error E).
+
+Definition parser_map {A B I E} (f: A -> B) (p: @parser A I E) : @parser B I E :=
+  fun s =>
+    let* (x, rest) := p s in
+    Ok (f x, rest).
+
+Definition maybe {A I E} (p: @parser A I E) : @parser (option A) I E :=
+  fun s =>
+    match p s with
+    | Ok (x, rest) => Ok (Some x, rest)
+    | Err _        => Ok (None, s)
+    end.
+
+Fixpoint any_aux {A I E} (parsers: list (@parser A I E)) (errs: @error E) : @parser A I E :=
+  fun s =>
+    match parsers with
+    | [] => Err errs
+    | p :: rest =>
+        match p s with
+        | Err err => any_aux rest (Both err errs) s
+        | Ok p => Ok p
+        end
+    end.
+
+Definition any {A I E} (parsers : list (@parser A I E)): @parser A I E := any_aux parsers NoError.
+
+Definition predicate {I E} (pred: I -> bool) (err: option I -> E) : @parser I I E :=
+  fun s => 
+    match s with
+    | [] => Err (Error (err None))
+    | c :: rest =>
+        match pred c with
+        | true => Ok (c, rest)
+        | false => Err (Error (err (Some c)))
+        end
+    end.
+
+Fixpoint many_aux { A I E} (p: @parser A I E) (fuel: nat) : @parser (list A) I E :=
+  fun s => 
+    match fuel with
+    | 0 => Ok ([], s)
+    | S fuel' =>
+        match p s with
+        | Err _ => Ok ([], s)
+        | Ok (val, rest) =>
+            let* (vals, rest) := many_aux p fuel' rest in
+            Ok (val :: vals, rest)
+        end
+    end.
+
+Definition many {A I E} (p: @parser A I E): @parser (list A) I E :=
+  fun s => many_aux p (S (length s)) s.
+
+(* Fixpoint repeat_n {T I E} (n: nat) (p: @parser T I E) : @parser (Vector.t T n) I E := *)
+(*   fun s => *)
+(*     match n with *)
+(*     | 0 => Ok (nil T, s) *)
+(*     | S n' => *)
+(*         let* (val, rest) := p s in *)
+(*         let* (vals, rest) := repeat_n n' p rest in *)
+(*         Ok (cons T val n' vals, rest) *)
+(*     end. *)
