json/Theorems/Json.v
@@ -1,0 +1,31 @@
+Require Import parser.
+
+From Coq Require Import Strings.String.
+From Coq Require Import ZArith.
+From Coq Require Import Lia.
+From Coq Require Import Lists.List. Import ListNotations.
+
+(* Theorem parse_null_isomorphic : parse_null "null" = Ok((JNull, "")). *)
+(*   reflexivity. *)
+(* Qed. *)
+(* Theorem parse_true_isomorphic : parse_true "true" = Ok((JTrue, "")). *)
+(*   reflexivity. *)
+(* Qed. *)
+(* Theorem parse_false_isomorphic : parse_false "false" = Ok((JFalse, "")). *)
+(*   reflexivity. *)
+(* Qed. *)
+
+
+(* Theorem parse_number_isomorphic :forall n, parse_number (serialize_json (JNumber n)) = Ok((JNumber n, "")). *)
+(* Proof. *)
+(*   intros. *)
+(*   unfold parse_number, serialize_json. *)
+(*   rewrite parser_map_correct. *)
+(*   rewrite parse_nat_isomorphic. *)
+(*   reflexivity. *)
+(* Defined. *)
+
+(* Theorem parse_correct_left (j: json) : parse_json (serialize_json j) = Ok((j, "")). *)
+(* Proof. *)
+(*   induction j; try auto. *)
+(*   - unfold parse_json. unfold one_of. rewrite parse_number_isomorphic. reflexivity. *)
