json/Theorems/Parser.v
@@ -1,0 +1,23 @@
+Require Import Json.Parser.
+
+Lemma parser_map_correct: forall T R I E (f: T -> R) s (p: @parser T I E),
+    (parser_map f p) s = fmap (fun '(v, rest) => (f v, rest)) (p s).
+Proof.
+  intros.
+  unfold parser_map, fmap.
+  destruct (p s) as [[val rest] |  err]; reflexivity.
+Defined.
+
+Lemma predicate_correct: forall T I E (p: @parser T I E) (pred: I -> bool) (err_handler: option I -> list E) v s rest,
+    Ok (v, rest) = predicate pred err_handler s ->
+    pred v = true.
+Proof.
+  intros.
+  unfold predicate in H.
+  
+  destruct s.
+  - discriminate H.
+  - destruct (pred i) eqn:Eq.
+    + inversion H. apply Eq.
+    + discriminate H.
+Defined.
